$a_{n+m} = \Sigma_{i=0}^{m-1}b_ia_{n+i}$ は、

$$
\left(\begin{matrix}a_{n+m}\\a_{n+m-1}\\\vdots\\a_{n+1}\end{matrix}\right)=\left(\begin{matrix}b_{m-1} & \cdots& b_1 & b_0\\1 & \cdots & 0 & 0\\\vdots & \ddots & \vdots & \vdots\\0 & \cdots & 1 & 0\end{matrix}\right)\left(\begin{matrix}a_{n+m-1}\\a_{n+m-2}\\\vdots\\a_{n}\end{matrix}\right)
$$

$a_{n+m} = \Sigma_{i=0}^{m-1}b_ia_{n+i}+c$ は、

$$
\left(\begin{matrix}a_{n+m}\\a_{n+m-1}\\\vdots\\a_{n+1}\\1\end{matrix}\right)=\left(\begin{matrix}b_{m-1} & \cdots& b_1 & b_0 & c\\1 & \cdots & 0 & 0 & 0\\\vdots & \ddots & \vdots & \vdots & \vdots\\0 & \cdots & 1 & 0 & 0\\0 & \cdots & 0 & 0 & 1\end{matrix}\right)\left(\begin{matrix}a_{n+m-1}\\a_{n+m-2}\\\vdots\\a_{n}\\1\end{matrix}\right)
$$
